First attempt at a proof technique for leader election

examples/Messaging/Election.v
@@ -3,9 +3,9 @@ From ITree Require Import
      CategoryOps
      Indexed.Sum.
 
-From Coq Require Import Nat List.
-
 From Coq Require Import
+     Nat
+     Lia
      Vector
      List
      Arith.PeanoNat.
@@ -14,6 +14,7 @@ From ITree Require Import
      CategoryOps.
 
 From ExtLib Require Import
+     Structures.Monad
      Structures.MonadState
      Data.Monads.StateMonad.
 
@@ -23,7 +24,8 @@ From CTree Require Import
      Interp.Preempt
      Interp.Network
      Logic.Kripke
-     Logic.Ctl.
+     Logic.Ctl
+     Misc.Vectors.
 
 From Equations Require Import Equations.
 
@@ -39,27 +41,27 @@ Variant message :=
   | Elected (u: nat).
 
 (*| Client process |*)
-Definition proc (id: uid)(n: nat): ctree (netE message +' parE) B01 unit :=
+Definition proc (id: uid)(n: nat): ctree (netE message) B01 unit :=
   let right := modulo (S id) n in
   (* 1. Send my [id] to the process on the right *)
-  send right (Candidate id);;
+  send id right (Candidate id);;
   (* 2. Loop until we know the leader *)
   CTree.iter
     (fun _ =>
-       m <- recv;;
+       m <- recv id;;
        match m with
        | Some (Candidate candidate) =>
            match Nat.compare candidate id with (* candidate < id *)
            (* My [left] neighbor proposed a candidate, I support that candidate *)
-           | Gt => send right (Candidate candidate) ;; Ret (inl tt)
+           | Gt => send id right (Candidate candidate) ;; Ret (inl tt)
            (* My left neighbor proposed a candidate, I do not support him *)
            | Lt => Ret (inl tt)
            (* I am the leader, but only I know *)
-           | Eq => send right (Elected id) ;; Ret (inr tt)
+           | Datatypes.Eq => send id right (Elected id) ;; Ret (inr tt)
            end
        | Some (Elected x) =>
            (* I know [x] is the leader *)
-           send right (Elected x) ;; Ret (inr tt)
+           send id right (Elected x) ;; Ret (inr tt)
        | None => Ret (inl tt) (* Didn't receive anything *)
        end) tt.
 
@@ -116,12 +118,165 @@ exists j, V /\ I ==> AX (proc j) |- V décroit strict
 ----------------------------------------------------
 V ==> AF (sched n proc) |- V décroit strict
 
+
  *)
 
-(*| The mailbox of the leader will eventually have a message that he was elected. |*)
-Lemma election_live:
-  <( {rr [proc 0 3; proc 1 3; proc 2 3]},
-     {([]%list, 0)} |= AG (AF now {(fun '(qs,id) => nth_error qs id = Some [Elected id]%list)}))>.
+Section Fair.
+  Context {E C : Type -> Type} {X : Type} `{HasB0: B0 -< C} (n : nat).
+  Variable sched : vec n (ctree E C X) -> ctree E C X.
+
+  (* Transitions of the scheduled ctree are necessarily taken from
+     the individual processes *)
+  Definition sched_correct := forall v l T',
+    trans l (sched v) T' ->
+    exists (i : fin n) t',
+    trans l (Vector.nth v i) t' /\ T' ≅ sched (replace v i t').
+
+  (* Process i will make some progress in finite time *)
+  Inductive sched_fair1_ i : vec n (ctree E C X) -> Prop :=
+  | sched_fair1_now : forall v,
+    ((exists l T', trans l (sched v) T') /\
+      forall l T', trans l (sched v) T' -> exists t', T' ≅ (sched (replace v i t'))) ->
+    sched_fair1_ i v
+  | sched_fair1_later : forall v,
+    (exists l T', trans l (sched v) T') /\
+    (forall l v',
+      trans l (sched v) (sched v') ->
+      sched_fair1_ i v') ->
+    sched_fair1_ i v.
+
+  (* Any process that can progress will do so in finite time *)
+  Definition sched_fair1 v :=
+    forall l t' i, trans l (Vector.nth v i) t' -> sched_fair1_ i v.
+
+  Program Definition sched_fairF : mon (vec n (ctree E C X) -> Prop) :=
+    {| body R v := sched_fair1 v /\ forall l v', trans l (sched v) (sched v') -> R v' |}.
+  Next Obligation.
+    split; auto. intros. apply H. now apply H1 in H2.
+  Qed.
+
+  (* Whenever a process can progress, it will do so in finite time *)
+  Definition sched_fair := forall v, (gfp sched_fairF) v.
+End Fair.
+
+Definition from_to_ (i j : nat) : nat -> Prop :=
+  fun k => Nat.le i k /\ Nat.lt k j.
+
+Definition from_to {n} (i j : fin n) : fin n -> Prop :=
+  fun k =>
+    let i := proj1_sig (Fin.to_nat i) in
+    let j := proj1_sig (Fin.to_nat j) in
+    let k := proj1_sig (Fin.to_nat k) in
+    (Nat.le i j -> from_to_ i j k) /\
+    (Nat.lt j i -> from_to_ j n k /\ from_to_ 0 i k).
+
+Variant candidate_state : Type :=
+| CandBegin
+| CandTraveling (d: nat)
+| CandLost.
+
+Variant election_state : Type :=
+| VCandidates (l: list candidate_state)
+| VElected (i: nat) (* i => i hops *)
+.
+Arguments election_state : clear implicits.
+
+Definition ids_wf {n} (ids : vec n nat) :=
+  forall j k, j <> k -> Vector.nth ids j <> Vector.nth ids k.
+
+Definition max_id {n} (ids : vec n nat) (wf : ids_wf ids) : fin n.
+Admitted.
+
+Lemma max_id_correct : forall {n} (ids : vec n nat) (wf : ids_wf ids),
+  forall k, k <> max_id wf -> Vector.nth ids k < Vector.nth ids (max_id wf).
+Admitted.
+
+(* Invariant during phase 1 (Candidate messages) *)
+Program Definition election_invariant_candidates n (ids : vec (S n) nat) (wf : ids_wf ids)
+  (cand_progress : list candidate_state) qs :=
+  List.length cand_progress = S n /\
+  List.nth (proj1_sig (Fin.to_nat (max_id wf))) cand_progress CandLost <> CandLost /\
+  forall i (Hi : (i < S n)%nat),
+    (List.nth_error cand_progress i = Some CandBegin \/ List.nth_error cand_progress i = Some CandLost) ->
+      ~ In (Candidate i) (concat qs) /\
+    forall p, List.nth_error cand_progress i = Some (CandTraveling p) ->
+      let i' := Fin.of_nat_lt Hi in
+      let j := (i + p + 1) mod (S n) in
+      (In (Candidate n) (List.nth j qs []%list)) /\
+      (forall k, from_to i' (Fin.of_nat_lt (p := j) _) k ->
+        Vector.nth ids k < Vector.nth ids i' /\
+        (i' = max_id wf -> k <> i' -> List.nth_error cand_progress (proj1_sig (Fin.to_nat k)) = Some CandLost)).
+Next Obligation.
+  lia.
+Qed.
+
+(* Invariant during phase 2 (Elected message) *)
+Definition election_invariant_elected n (ids : vec (S n) nat) (wf : ids_wf ids)
+  (elected_progress : nat) (qs: list (list message)) :=
+  forall (He : elected_progress < n),
+  let m := proj1_sig (Fin.to_nat (max_id wf)) in
+  let e' := Fin.of_nat_lt He in
+  let j := (m + elected_progress + 1) mod (S n) in
+  List.nth j qs []%list = [Elected m]%list /\
+  forall k, k <> j -> List.nth k qs []%list = []%list.
+
+Definition election_invariant n (ids : vec (S n) nat) (wf : ids_wf ids) st qs :=
+  match st with
+  | VCandidates l => election_invariant_candidates wf l qs
+  | VElected n => election_invariant_elected wf n qs
+  end.
+
+Definition handle_election_state n (qs: list (list message)) (st: election_state) :
+  forall X, netE message X -> election_state :=
+  fun X e =>
+  match e with
+  | Send i to msg =>
+    match st, msg with
+    | VCandidates l, Candidate c =>
+      VCandidates (nth_map (fun i =>
+        match i with
+        | CandBegin => CandTraveling 0
+        | CandTraveling d => CandTraveling (S d)
+        | _ => CandLost
+        end)
+        l c)
+    | VCandidates l, Elected e => VElected 0
+    | VElected i, Elected e => VElected (S i)
+    | _, _ => VCandidates (List.repeat CandLost n)
+    end
+  | _ => st
+  end.
+
+Lemma ktrans_trans : forall {E C X St h} `{B0 -< C} (s s' : St) (t t' : ctree E C X),
+  ktrans (h := h) (t, s) (t', s') ->
+  exists l, trans l t t'.
 Proof.
-  next.
+  intros. inversion H0; subst; eauto. (* wrong in the Ret case *)
+Admitted.
+
+Theorem distr_system_dec_variant : forall {n C X St Msg} `{HasB0: B0 -< C}
+  (h : list (list Msg) -> St -> forall X, netE Msg X -> St)
+  (Inv : vec n (ctree (netE Msg) C X) -> list (list Msg) -> St -> Prop) (var : St -> nat)
+  (sched : vec n (ctree (netE Msg) C X) -> ctree (netE Msg) C X)
+  (Hc : sched_correct sched) (Hf : sched_fair (HasB0 := HasB0) sched)
+  (Hprog : forall v qs st, Inv v qs st -> var st > 0 -> ~is_stuck (sched v))
+  (Hdec : forall v qs st, Inv v qs st -> var st > 0 ->
+    forall v' qs' st', ktrans (h := handler_netE h) (sched v, (qs, st)) (sched v', (qs', st')) ->
+    Inv v' qs' st' /\ var st' < var st),
+  forall v qs st, Inv v qs st -> entailsF (h := handler_netE h) <(AF (now {(fun '(qs, st) => var st = 0)}))> (sched v) (qs, st).
+Proof.
+  intros. cbn.
+  remember (var st) as i. assert (var st <= i)%nat by lia. clear Heqi.
+  revert v qs st H H0. induction i; intros.
+  - left. lia.
+  - inversion H0. 2: { apply IHi; auto. }
+    right. apply I. intros. apply ktrans_trans in H1 as ?. destruct H3.
+    apply Hc in H3 as (? & ? & ? & ?).
+    rewrite H4 in H1.
+    cbn in Hdec. destruct s'.
+    unshelve epose proof (Hdec _ _ _ _ _ _ _ _ H1) as []; auto.
+    lia.
+    assert (var s <= i)%nat by lia.
+    replace t' with (sched (replace v x0 x1)) by admit.
+    apply IHi; auto.
 Admitted.
